in-place merge sort on slices

pulse/lib/pulse/lib/Pulse.Lib.Sort.Merge.Slice.fst
@@ -1,13 +1,14 @@
-module Pulse.Lib.Sort.Merge.Array
+module Pulse.Lib.Sort.Merge.Slice
 #lang-pulse
 open Pulse.Lib.Pervasives
 include Pulse.Lib.Sort.Base
 include Pulse.Lib.Sort.Merge.Spec
-include Pulse.Lib.Array
+include Pulse.Lib.Slice.Util
 open Pulse.Lib.Sort.Merge.Common
 
 module SM = Pulse.Lib.SeqMatch.Util
-module AS = Pulse.Lib.Swap.Array
+module S = Pulse.Lib.Slice.Util
+module AS = Pulse.Lib.Swap.Slice
 module SZ = FStar.SizeT
 module R = Pulse.Lib.Reference
 module Trade = Pulse.Lib.Trade.Util
@@ -16,32 +17,31 @@ module I16 = FStar.Int16
 let merge_invariant_prop
     (#t: Type)
     (compare: t -> t -> int)
-    (lo: SZ.t)
-    (hi: SZ.t)
+    (len: SZ.t)
     (l1_0: Ghost.erased (list t))
     (l2_0: Ghost.erased (list t))
     (cont: bool)
     i1 i2 (res: bool) accu l1 l2
 : Tot prop
 =
-            SZ.v lo <= SZ.v i1 /\
             SZ.v i1 <= SZ.v i2 /\
-            SZ.v i2 <= SZ.v hi /\
+            SZ.v i2 <= SZ.v len /\
+            SZ.v i1 == List.Tot.length accu /\
+            SZ.v i2 - SZ.v i1 == List.Tot.length l1 /\
+            SZ.v len - SZ.v i2 == List.Tot.length l2 /\
             spec_merge compare [] l1_0 l2_0 == (
                 if res
                 then spec_merge compare accu l1 l2
                 else (false, accu `List.Tot.append` (l1 `List.Tot.append` l2))
             ) /\
-            cont == (res && not (i1 = i2 || i2 = hi))
+            cont == (res && not (i1 = i2 || i2 = len))
 
-let merge_invariant // FIXME: WHY WHY WHY?
+let merge_invariant
     (#tl #th: Type)
     (vmatch: tl -> th -> slprop)
     (compare: th -> th -> int)
-    (a: array tl)
+    (a: slice tl)
     (c1_0 c2_0: (Seq.seq tl))
-    (lo: SZ.t)
-    (hi: SZ.t)
     (l1_0: (list th))
     (l2_0: (list th))
     (pi1: R.ref SZ.t)
@@ -50,18 +50,53 @@ let merge_invariant // FIXME: WHY WHY WHY?
     (cont: bool)
     i1 i2 (res: bool) c c1 c2 accu l1 l2
 : Tot slprop
-=
+= exists* ca .
         R.pts_to pi1 i1 ** R.pts_to pi2 i2 ** R.pts_to pres res **
-        pts_to_range a (SZ.v lo) (SZ.v i1) c **
+        pts_to a ca **
         SM.seq_list_match c accu vmatch **
-        pts_to_range a (SZ.v i1) (SZ.v i2) c1 **
         SM.seq_list_match c1 l1 vmatch **
-        pts_to_range a (SZ.v i2) (SZ.v hi) c2 **
         SM.seq_list_match c2 l2 vmatch **
         Trade.trade
           (SM.seq_list_match c accu vmatch ** (SM.seq_list_match c1 l1 vmatch ** SM.seq_list_match c2 l2 vmatch))
           (SM.seq_list_match c1_0 l1_0 vmatch ** SM.seq_list_match c2_0 l2_0 vmatch) **
-        pure (merge_invariant_prop compare lo hi l1_0 l2_0 cont i1 i2 res accu l1 l2)
+        pure (ca == (Seq.append c (Seq.append c1 c2))) **
+        pure (merge_invariant_prop compare (S.len a) l1_0 l2_0 cont i1 i2 res accu l1 l2)
+
+let merge_case_1
+  (#t: Type)
+  (c: Seq.seq t)
+  (x1: t)
+  (c1' c2': Seq.seq t)
+: Lemma
+  (requires Seq.length c1' > 0 /\ x1 == Seq.head c1')
+  (ensures (
+    Seq.append c (Seq.append c1' c2') `Seq.equal` Seq.append (Seq.append c (Seq.cons x1 Seq.empty)) (Seq.append (Seq.tail c1') c2')
+  ))
+= ()
+
+let merge_case_2_pre
+  (#t: Type)
+  (c c1': Seq.seq t)
+  (x2: t)
+  (c2': Seq.seq t)
+: Lemma
+  (requires Seq.length c2' > 0 /\ x2 == Seq.head c2')
+  (ensures (
+    Seq.append c (Seq.append c1' c2') `Seq.equal` Seq.append (Seq.append c (Seq.append c1' (Seq.cons x2 Seq.empty))) (Seq.tail c2')
+  ))
+= ()
+
+let merge_case_2_post
+  (#t: Type)
+  (c c1': Seq.seq t)
+  (x2: t)
+  (c2': Seq.seq t)
+: Lemma
+  (requires Seq.length c2' > 0 /\ x2 == Seq.head c2')
+  (ensures (
+    Seq.append (Seq.append c (Seq.cons x2 Seq.empty)) (Seq.append c1' (Seq.tail c2')) `Seq.equal` Seq.append (Seq.append c (Seq.append (Seq.cons x2 Seq.empty) c1')) (Seq.tail c2')  
+  ))
+= ()
 
 inline_for_extraction
 fn merge
@@ -69,80 +104,73 @@ fn merge
     (vmatch: tl -> th -> slprop)
     (compare: Ghost.erased (th -> th -> int))
     (impl_compare: impl_compare_t vmatch compare)
-    (a: array tl)
-    (lo: SZ.t)
+    (a: S.slice tl)
     (mi: SZ.t)
-    (hi: SZ.t)
-    (#c1: Ghost.erased (Seq.seq tl))
-    (#c2: Ghost.erased (Seq.seq tl))
+    (c1: Ghost.erased (Seq.seq tl))
+    (c2: Ghost.erased (Seq.seq tl))
     (#l1_0: Ghost.erased (list th))
     (#l2_0: Ghost.erased (list th))
 requires
-    pts_to_range a (SZ.v lo) (SZ.v mi) c1 **
-    pts_to_range a (SZ.v mi) (SZ.v hi) c2 **
+    pts_to a (Seq.append c1 c2) **
     SM.seq_list_match c1 l1_0 vmatch **
-    SM.seq_list_match c2 l2_0 vmatch
+    SM.seq_list_match c2 l2_0 vmatch **
+    pure (SZ.v mi == Seq.length c1)
 returns res: bool
 ensures exists* c l .
-    pts_to_range a (SZ.v lo) (SZ.v hi) c **
+    pts_to a c **
     SM.seq_list_match c l vmatch **
     Trade.trade
       (SM.seq_list_match c l vmatch)
       (SM.seq_list_match c1 l1_0 vmatch ** SM.seq_list_match c2 l2_0 vmatch) **
     pure (
-        spec_merge compare [] l1_0 l2_0 == (res, l)
+        spec_merge compare [] l1_0 l2_0 == (res, l) /\
+        List.Tot.length l == List.Tot.length l1_0 + List.Tot.length l2_0
     )
 {
-    let mut pi1 = lo;
-    pts_to_range_prop a #(SZ.v lo) #(SZ.v mi);
-    pts_to_range_prop a #(SZ.v mi) #(SZ.v hi);
-    pts_to_range_split a (SZ.v lo) (SZ.v lo) (SZ.v mi);
-    with c1l . assert (pts_to_range a (SZ.v lo) (SZ.v lo) c1l);
-    with c1r . assert (pts_to_range a (SZ.v lo) (SZ.v mi) c1r);
-    assert (pure (Seq.equal c1r c1));
-    rewrite (pts_to_range a (SZ.v lo) (SZ.v mi) c1r) as (pts_to_range a (SZ.v lo) (SZ.v mi) c1);
+    S.pts_to_len a;
+    let mut pi1 = 0sz;
+    SM.seq_list_match_length vmatch c1 l1_0;
+    SM.seq_list_match_length vmatch c2 l2_0;
+    Seq.append_empty_l (Seq.append c1 c2);
+    rewrite (pts_to a (Seq.append c1 c2)) as (pts_to a (Seq.append Seq.empty (Seq.append c1 c2)));
     Trade.refl (SM.seq_list_match c1 l1_0 vmatch ** SM.seq_list_match c2 l2_0 vmatch);
-    SM.seq_list_match_nil_intro_trade c1l [] vmatch (SM.seq_list_match c1 l1_0 vmatch ** SM.seq_list_match c2 l2_0 vmatch) (SM.seq_list_match c1 l1_0 vmatch ** SM.seq_list_match c2 l2_0 vmatch);
-    SM.seq_list_match_nil_intro c1l [] vmatch;
+    SM.seq_list_match_nil_intro_trade Seq.empty [] vmatch (SM.seq_list_match c1 l1_0 vmatch ** SM.seq_list_match c2 l2_0 vmatch) (SM.seq_list_match c1 l1_0 vmatch ** SM.seq_list_match c2 l2_0 vmatch);
+    SM.seq_list_match_nil_intro Seq.empty [] vmatch;
     let mut pi2 = mi;
     let mut pres = true;
-    fold (merge_invariant vmatch compare a c1 c2 lo hi l1_0 l2_0 pi1 pi2 pres
-        (not (lo = mi || mi = hi))
-        lo mi true
-        c1l c1 c2 [] l1_0 l2_0
+    fold (merge_invariant vmatch compare a c1 c2 l1_0 l2_0 pi1 pi2 pres
+        (not (0sz = mi || mi = S.len a))
+        0sz mi true
+        Seq.empty c1 c2 [] l1_0 l2_0
     );
     while (
         with gcont gi1 gi2 gres c c1' c2' accu l1' l2' .
-            assert (merge_invariant vmatch compare a c1 c2 lo hi l1_0 l2_0 pi1 pi2 pres gcont gi1 gi2 gres c c1' c2' accu l1' l2');
-        unfold (merge_invariant vmatch compare a c1 c2 lo hi l1_0 l2_0 pi1 pi2 pres gcont gi1 gi2 gres c c1' c2' accu l1' l2');
+            assert (merge_invariant vmatch compare a c1 c2 l1_0 l2_0 pi1 pi2 pres gcont gi1 gi2 gres c c1' c2' accu l1' l2');
+        unfold (merge_invariant vmatch compare a c1 c2 l1_0 l2_0 pi1 pi2 pres gcont gi1 gi2 gres c c1' c2' accu l1' l2');
         let i1 = !pi1;
         let i2 = !pi2;
         let res = !pres;
-        let cont = (res && not (i1 = i2 || i2 = hi));
-        fold (merge_invariant vmatch compare a c1 c2 lo hi l1_0 l2_0 pi1 pi2 pres cont gi1 gi2 gres c c1' c2' accu l1' l2');
+        let cont = (res && not (i1 = i2 || i2 = S.len a));
+        fold (merge_invariant vmatch compare a c1 c2 l1_0 l2_0 pi1 pi2 pres cont gi1 gi2 gres c c1' c2' accu l1' l2');
         cont
     )
     invariant cont . exists* i1 i2 res c c1' c2' accu l1' l2' .
-        merge_invariant vmatch compare a c1 c2 lo hi l1_0 l2_0 pi1 pi2 pres cont i1 i2 res c c1' c2' accu l1' l2'
+        merge_invariant vmatch compare a c1 c2 l1_0 l2_0 pi1 pi2 pres cont i1 i2 res c c1' c2' accu l1' l2'
     {
         with gi1 gi2 gres c c1' c2' accu l1 l2 .
-            assert (merge_invariant vmatch compare a c1 c2 lo hi l1_0 l2_0 pi1 pi2 pres true gi1 gi2 gres c c1' c2' accu l1 l2);
-        unfold (merge_invariant vmatch compare a c1 c2 lo hi l1_0 l2_0 pi1 pi2 pres true gi1 gi2 gres c c1' c2' accu l1 l2);
+            assert (merge_invariant vmatch compare a c1 c2 l1_0 l2_0 pi1 pi2 pres true gi1 gi2 gres c c1' c2' accu l1 l2);
+        unfold (merge_invariant vmatch compare a c1 c2 l1_0 l2_0 pi1 pi2 pres true gi1 gi2 gres c c1' c2' accu l1 l2);
         let prf_res : squash (gres == true) = ();
+        S.pts_to_len a;
+        SM.seq_list_match_length vmatch c accu;
         SM.seq_list_match_length vmatch c1' l1;
         SM.seq_list_match_length vmatch c2' l2;
-        pts_to_range_prop a #(SZ.v gi1) #(SZ.v gi2);
-        pts_to_range_prop a #(SZ.v gi2) #(SZ.v hi);
         let prf1 = SM.seq_list_match_cons_elim_trade c1' l1 vmatch;
         let prf2 = SM.seq_list_match_cons_elim_trade c2' l2 vmatch;
         let i1 = !pi1;
-        rewrite (pts_to_range a (SZ.v gi1) (SZ.v gi2) c1') // FIXME: WHY WHY WHY?
-            as (pts_to_range a (Ghost.reveal (SZ.v gi1)) (Ghost.reveal (SZ.v gi2)) c1');
-        let x1 = pts_to_range_index a i1 #(SZ.v gi1) #(SZ.v gi2);
+        let x1 = S.op_Array_Access a i1;
         let i2 = !pi2;
-        rewrite (pts_to_range a (SZ.v gi2) (SZ.v hi) c2') // FIXME: WHY WHY WHY?
-            as (pts_to_range a (Ghost.reveal (SZ.v gi2)) (Ghost.reveal (SZ.v hi)) c2');
-        let x2 = pts_to_range_index a i2 #(SZ.v gi2) #(SZ.v hi);
+        let x2 = S.op_Array_Access a i2;
         Trade.rewrite_with_trade (vmatch (Seq.head c1') (List.Tot.hd l1))
             (vmatch x1 (List.Tot.hd l1));
         Trade.trans_hyp_l (vmatch x1 (List.Tot.hd l1)) _ _ _;
@@ -158,31 +186,28 @@ ensures exists* c l .
         Trade.elim (vmatch x2 (List.Tot.hd l2) ** _) _;
         if (comp = 0s) {
             pres := false;
-            fold (merge_invariant vmatch compare a c1 c2 lo hi l1_0 l2_0 pi1 pi2 pres false gi1 gi2 false c
+            fold (merge_invariant vmatch compare a c1 c2 l1_0 l2_0 (* pc pc1 pc2 *) pi1 pi2 pres false gi1 gi2 false c
                 c1'
                 c2'
                 accu
                 l1
                 l2
             )
-        } else if (comp `I16.lt` 0s) {
+        }
+        else if (comp `I16.lt` 0s) {
             let i1' = SZ.add i1 1sz;
             pi1 := i1';
-            pts_to_range_split a (Ghost.reveal (SZ.v gi1)) (SZ.v i1') (Ghost.reveal (SZ.v gi2));
             let _p : squash (Seq.head c1' == x1) = ();
             let prf_c1' : squash (Seq.slice c1' 0 1 `Seq.equal` Seq.cons x1 Seq.empty) =
               seq_helper_1 c1' x1;
-            rewrite (pts_to_range a (Ghost.reveal (SZ.v gi1)) (SZ.v i1') (Seq.slice c1' 0 (SZ.v i1' - SZ.v gi1)))
-                as (pts_to_range a (SZ.v gi1) (SZ.v i1') (Seq.cons x1 Seq.empty));
-            pts_to_range_join a (SZ.v lo) (SZ.v gi1) (SZ.v i1');
             merge_aux_consume_1 vmatch c accu c1' l1 c2' l2 x1 ();
             Trade.trans _ _ (SM.seq_list_match c1 l1_0 vmatch ** SM.seq_list_match c2 l2_0 vmatch);
-            rewrite (pts_to_range a (Ghost.reveal (SZ.v gi2)) (Ghost.reveal (SZ.v hi)) c2')
-                as (pts_to_range a (SZ.v gi2) (SZ.v hi) c2');
-            rewrite (pts_to_range a (SZ.v i1') (Ghost.reveal (SZ.v gi2)) (Seq.tail c1'))
-                as (pts_to_range a (SZ.v i1') (SZ.v gi2) (Seq.tail c1'));
-            let gcont' = Ghost.hide (gres && not (i1' `size_eq` gi2 || gi2 `size_eq` hi));
-            fold (merge_invariant vmatch compare a c1 c2 lo hi l1_0 l2_0 pi1 pi2 pres gcont' i1' gi2 gres
+            let gcont' = Ghost.hide (gres && not (i1' `size_eq` gi2 || gi2 `size_eq` S.len a));
+            List.Tot.append_assoc accu l1 l2;
+            List.Tot.append_assoc accu [List.Tot.hd l1] (List.Tot.tl l1);
+            List.Tot.append_assoc (List.Tot.append accu [List.Tot.hd l1]) (List.Tot.tl l1) l2;
+            merge_case_1 c x1 c1' c2';
+            fold (merge_invariant vmatch compare a c1 c2 l1_0 l2_0 pi1 pi2 pres gcont' i1' gi2 gres
                 (Seq.append c (Seq.cons x1 Seq.empty))
                 (Seq.tail c1')
                 c2'
@@ -192,24 +217,26 @@ ensures exists* c l .
             )
         } else {
             let i2' = SZ.add i2 1sz;
-            rewrite (pts_to_range a (Ghost.reveal (SZ.v gi1)) (Ghost.reveal (SZ.v gi2)) c1')
-                as (pts_to_range a (SZ.v i1) (SZ.v i2) (Seq.cons x1 (Seq.tail c1')));
             let prf_c2' : squash (Seq.slice c2' 0 1 `Seq.equal` Seq.cons x2 Seq.empty) = seq_helper_1 c2' x2;
-            pts_to_range_split a (Ghost.reveal (SZ.v gi2)) (SZ.v i2') (Ghost.reveal (SZ.v hi));
-            rewrite (pts_to_range a (Ghost.reveal (SZ.v gi2)) (SZ.v i2') (Seq.slice c2' 0 1))
-                as (pts_to_range a (SZ.v i2) (SZ.v i2') (Seq.cons x2 Seq.empty));
-            rewrite (pts_to_range a (SZ.v i2') (Ghost.reveal (SZ.v hi)) (Seq.tail c2'))
-                as (pts_to_range a (SZ.v i2') (SZ.v hi) (Seq.tail c2'));
-            let i1' = AS.array_swap a i1 i2' i2;
-            rewrite (pts_to_range a (SZ.v lo) (SZ.v gi1) c)
-                as (pts_to_range a (SZ.v lo) (SZ.v i1) c);
-            pts_to_range_join a (SZ.v lo) (SZ.v i1) (SZ.v i1');
+            merge_case_2_pre c c1' x2 c2';
+            let Mktuple2 ac01 ac2 = S.append_split a i2' #(Seq.append c (Seq.append c1' (Seq.cons x2 Seq.empty))) #(Seq.tail c2');
+            let Mktuple2 ac ac1 = S.append_split ac01 i1 #c #(Seq.append c1' (Seq.cons x2 Seq.empty));
+            AS.slice_swap' ac1 (SZ.sub i2 i1) c1' (Seq.cons x2 Seq.empty);
+            S.join ac ac1 ac01;
+            S.join ac01 ac2 a;
+            merge_case_2_post c c1' x2 c2';
+            let i1' = SZ.add i1 1sz;
             pi1 := i1';
             pi2 := i2';
             merge_aux_consume_2 vmatch c accu c1' l1 c2' l2 x2 ();
             Trade.trans _ _ (SM.seq_list_match c1 l1_0 vmatch ** SM.seq_list_match c2 l2_0 vmatch);
-            let gcont' = Ghost.hide (gres && not (i1' `size_eq` i2' || i2' `size_eq` hi));
-            fold (merge_invariant vmatch compare a c1 c2 lo hi l1_0 l2_0 pi1 pi2 pres gcont' i1' i2' gres
+            let gcont' = Ghost.hide (gres && not (i1' `size_eq` i2' || i2' `size_eq` S.len a));
+            List.Tot.append_assoc l1 [List.Tot.hd l2] (List.Tot.tl l2);
+            List.Tot.append_assoc accu (List.Tot.append l1 [List.Tot.hd l2]) (List.Tot.tl l2);
+            List.Tot.append_assoc accu l1 [List.Tot.hd l2];
+            List.Tot.append_assoc accu [List.Tot.hd l2] l1;
+            List.Tot.append_assoc (List.Tot.append accu [List.Tot.hd l2]) l1 (List.Tot.tl l2);
+            fold (merge_invariant vmatch compare a c1 c2 l1_0 l2_0 pi1 pi2 pres gcont' i1' i2' gres
                 (Seq.append c (Seq.cons x2 Seq.empty))
                 c1'
                 (Seq.tail c2')
@@ -220,18 +247,13 @@ ensures exists* c l .
         }
     };
     with i1 i2 res c c1' c2' accu l1' l2' .
-        assert (merge_invariant vmatch compare a c1 c2 lo hi l1_0 l2_0 pi1 pi2 pres false i1 i2 res c c1' c2' accu l1' l2');
-    unfold (merge_invariant vmatch compare a c1 c2 lo hi l1_0 l2_0 pi1 pi2 pres false i1 i2 res c c1' c2' accu l1' l2');
-    SM.seq_list_match_length vmatch c1' l1';
-    SM.seq_list_match_length vmatch c2' l2';
-    List.Tot.append_l_nil l1';
-    pts_to_range_prop a #(SZ.v i1) #(SZ.v i2);
-    pts_to_range_prop a #(SZ.v i2) #(SZ.v hi);
-    pts_to_range_join a (SZ.v i1) (SZ.v i2) (SZ.v hi);
+        assert (merge_invariant vmatch compare a c1 c2 l1_0 l2_0 pi1 pi2 pres false i1 i2 res c c1' c2' accu l1' l2');
+    unfold (merge_invariant vmatch compare a c1 c2 l1_0 l2_0 pi1 pi2 pres false i1 i2 res c c1' c2' accu l1' l2');
     SM.seq_list_match_append_intro_trade vmatch c1' l1' c2' l2';
+    List.Tot.append_length l1' l2';
     Trade.trans_hyp_r (SM.seq_list_match c accu vmatch) (SM.seq_list_match (Seq.append c1' c2') (List.Tot.append l1' l2') vmatch) (SM.seq_list_match c1' l1' vmatch ** SM.seq_list_match c2' l2' vmatch) _;
-    pts_to_range_join a (SZ.v lo) (SZ.v i1) (SZ.v hi);
     SM.seq_list_match_append_intro_trade vmatch c accu (c1' `Seq.append` c2') (l1' `List.Tot.append` l2');
+    List.Tot.append_length accu (List.Tot.append l1' l2');
     Trade.trans _ _ (SM.seq_list_match c1 l1_0 vmatch ** SM.seq_list_match c2 l2_0 vmatch);
     !pres
 }
@@ -240,21 +262,20 @@ let sort_aux_post
   (#tl #th: Type0)
   (vmatch: tl -> th -> slprop)
   (compare: th -> th -> int)
-    (a: array tl)
-    (lo: SZ.t)
-    (hi: SZ.t)
+    (a: S.slice tl)
     (c: Seq.seq tl)
     (l: list th)
     (res: bool)
 : Tot slprop
 = exists* (c': Seq.seq tl) (l': list th).
-    pts_to_range a (SZ.v lo) (SZ.v hi) c' **
+    pts_to a c' **
     SM.seq_list_match c' l' vmatch **
     Trade.trade
       (SM.seq_list_match c' l' vmatch)
       (SM.seq_list_match c l vmatch) **
     pure (
-        spec_sort compare l == (res, l')
+        spec_sort compare l == (res, l') /\
+        List.Tot.length l' == List.Tot.length l
     )
 
 inline_for_extraction
@@ -263,17 +284,15 @@ let sort_aux_t
   (vmatch: tl -> th -> slprop)
   (compare: th -> th -> int)
 =
-    (a: array tl) ->
-    (lo: SZ.t) ->
-    (hi: SZ.t) ->
+    (a: S.slice tl) ->
     (#c: Ghost.erased (Seq.seq tl)) ->
     (#l: Ghost.erased (list th)) ->
 stt bool
   (
-    pts_to_range a (SZ.v lo) (SZ.v hi) c **
+    pts_to a c **
     SM.seq_list_match c l vmatch
   )
-  (fun res -> sort_aux_post vmatch compare a lo hi c l res)
+  (fun res -> sort_aux_post vmatch compare a c l res)
 
 inline_for_extraction
 fn sort_aux
@@ -284,25 +303,24 @@ fn sort_aux
   (sort_aux: sort_aux_t #tl #th vmatch compare)
 : sort_aux_t #tl #th vmatch compare
 = 
-    (a: array tl)
-    (lo: SZ.t)
-    (hi: SZ.t)
+    (a: S.slice tl)
     (#c: Ghost.erased (Seq.seq tl))
     (#l: Ghost.erased (list th))
 {
-    pts_to_range_prop a;
+    S.pts_to_len a;
     SM.seq_list_match_length vmatch c l;
-    let len = hi `SZ.sub` lo;
+    let len = S.len a;
     if (len `SZ.lt` 2sz) {
         Trade.refl (SM.seq_list_match c l vmatch);
-        fold (sort_aux_post vmatch compare a lo hi c l true);
+        fold (sort_aux_post vmatch compare a c l true);
         true
     } else {
         let len_half = len `SZ.div` 2sz;
-        let mi = lo `SZ.add` len_half;
-        pts_to_range_split a (SZ.v lo) (SZ.v mi) (SZ.v hi);
-        with c1 . assert (pts_to_range a (SZ.v lo) (SZ.v mi) c1);
-        with c2 . assert (pts_to_range a (SZ.v mi) (SZ.v hi) c2);
+        let mi = len_half;
+        let Mktuple2 a1 a2 = S.split a mi;
+        Seq.lemma_split c (SZ.v mi);
+        with c1 . assert (pts_to a1 c1);
+        with c2 . assert (pts_to a2 c2);
         let l1l2 = Ghost.hide (List.Tot.splitAt (SZ.v len_half) l);
         let l1 = Ghost.hide (fst l1l2);
         let l2 = Ghost.hide (snd l1l2);
@@ -310,31 +328,36 @@ fn sort_aux
           (SM.seq_list_match (c1 `Seq.append` c2) (l1 `List.Tot.append` l2) vmatch);
         SM.seq_list_match_append_elim_trade vmatch c1 l1 c2 l2;
         Trade.trans _ _ (SM.seq_list_match c l vmatch);
-        let res = sort_aux a lo mi;
-        unfold (sort_aux_post vmatch compare a lo mi c1 l1);
-        with c1' l1' . assert (pts_to_range a (SZ.v lo) (SZ.v mi) c1' ** SM.seq_list_match c1' l1' vmatch);
+        let res = sort_aux a1;
+        unfold (sort_aux_post vmatch compare a1 c1 l1);
+        with c1' l1' . assert (pts_to a1 c1' ** SM.seq_list_match c1' l1' vmatch);
+        SM.seq_list_match_length vmatch c1' l1';
         Trade.trans_hyp_l (SM.seq_list_match c1' l1' vmatch) (SM.seq_list_match c1 l1 vmatch) (SM.seq_list_match c2 l2 vmatch) (SM.seq_list_match c l vmatch);
         if (not res) {
-            pts_to_range_join a (SZ.v lo) (SZ.v mi) (SZ.v hi);
+            S.join a1 a2 a;
             SM.seq_list_match_append_intro_trade vmatch c1' l1' c2 l2;
             Trade.trans _ _ (SM.seq_list_match c l vmatch);
-            fold (sort_aux_post vmatch compare a lo hi c l false);
+            List.Tot.append_length l1'  l2;
+            fold (sort_aux_post vmatch compare a c l false);
             false
         } else {
-            let res = sort_aux a mi hi;
-            unfold (sort_aux_post vmatch compare a mi hi c2 l2);
-            with c2' l2' . assert (pts_to_range a (SZ.v mi) (SZ.v hi) c2' ** SM.seq_list_match c2' l2' vmatch);
+            let res = sort_aux a2;
+            unfold (sort_aux_post vmatch compare a2 c2 l2);
+            with c2' l2' . assert (pts_to a2 c2' ** SM.seq_list_match c2' l2' vmatch);
+            SM.seq_list_match_length vmatch c2' l2';
             Trade.trans_hyp_r (SM.seq_list_match c1' l1' vmatch) (SM.seq_list_match c2' l2' vmatch) (SM.seq_list_match c2 l2 vmatch) (SM.seq_list_match c l vmatch);
-            if (not res) {
-                pts_to_range_join a (SZ.v lo) (SZ.v mi) (SZ.v hi);
+            S.join a1 a2 a;
+            List.Tot.append_length l1'  l2';
+           if (not res) {
                 SM.seq_list_match_append_intro_trade vmatch c1' l1' c2' l2';
                 Trade.trans _ _ (SM.seq_list_match c l vmatch);
-                fold (sort_aux_post vmatch compare a lo hi c l false);
+                fold (sort_aux_post vmatch compare a c l false);
                 false
             } else {
-                let res = merge vmatch compare impl_compare a lo mi hi;
+                let res = merge vmatch compare impl_compare a mi c1' c2';
                 Trade.trans _ _ (SM.seq_list_match c l vmatch);
-                fold (sort_aux_post vmatch compare a lo hi c l res);
+                SM.seq_list_match_length vmatch _ _;
+                fold (sort_aux_post vmatch compare a c l res);
                 res
             }
         }
@@ -347,14 +370,12 @@ let sort_t
   (vmatch: tl -> th -> slprop)
   (compare: (th -> th -> int))
 =
-    (a: array tl) ->
-    (len: SZ.t) ->
+    (a: S.slice tl) ->
     (#c: Ghost.erased (Seq.seq tl)) ->
     (#l: Ghost.erased (list th)) ->
     stt bool
     (pts_to a c **
-      SM.seq_list_match c l vmatch **
-      pure (SZ.v len == length a \/ SZ.v len == Seq.length c \/ SZ.v len == List.Tot.length l)
+      SM.seq_list_match c l vmatch
     )
     (fun res -> exists* c' l' .
       pts_to a c' **
@@ -375,21 +396,13 @@ fn sort
   (sort_aux: sort_aux_t #tl #th vmatch compare)
 : sort_t #_ #_ vmatch compare
 =
-    (a: array tl)
-    (len: SZ.t)
+    (a: S.slice tl)
     (#c: Ghost.erased (Seq.seq tl))
     (#l: Ghost.erased (list th))
 {
-    pts_to_len a;
+    S.pts_to_len a;
     SM.seq_list_match_length vmatch c l;
-    pts_to_range_intro a 1.0R c;
-    rewrite (pts_to_range a 0 (length a) c)
-      as (pts_to_range a (SZ.v 0sz) (SZ.v len) c);
-    let res = sort_aux a 0sz len;
-    unfold (sort_aux_post vmatch compare a 0sz len c l res);
-    with c' . assert (pts_to_range a (SZ.v 0sz) (SZ.v len) c');
-    rewrite (pts_to_range a (SZ.v 0sz) (SZ.v len) c')
-        as (pts_to_range a 0 (length a) c');
-    pts_to_range_elim a 1.0R c';
+    let res = sort_aux a;
+    unfold (sort_aux_post vmatch compare a c l res);
     res
 }
